<?xml version="1.0"?>
<rdf:RDF xmlns="http://www.semanticweb.org/esther/ontologies/sys-self#"
     xml:base="http://www.semanticweb.org/esther/ontologies/sys-self"
     xmlns:owl="http://www.w3.org/2002/07/owl#"
     xmlns:rdf="http://www.w3.org/1999/02/22-rdf-syntax-ns#"
     xmlns:sys="http://www.semanticweb.org/esther/ontologies/sys-self#"
     xmlns:xml="http://www.w3.org/XML/1998/namespace"
     xmlns:xsd="http://www.w3.org/2001/XMLSchema#"
     xmlns:rdfs="http://www.w3.org/2000/01/rdf-schema#">
    <owl:Ontology rdf:about="http://www.semanticweb.org/esther/ontologies/sys-self">
        <owl:versionIRI rdf:resource="http://www.semanticweb.org/esther/ontologies/sys-self/1.0.0"/>
    </owl:Ontology>
    


    <!-- 
    ///////////////////////////////////////////////////////////////////////////////////////
    //
    // Object Properties
    //
    ///////////////////////////////////////////////////////////////////////////////////////
     -->

    


    <!-- http://www.semanticweb.org/esther/ontologies/sys-self#allocates -->

    <owl:ObjectProperty rdf:about="http://www.semanticweb.org/esther/ontologies/sys-self#allocates">
        <rdfs:domain rdf:resource="http://www.semanticweb.org/esther/ontologies/sys-self#Architecture"/>
        <rdfs:range rdf:resource="http://www.semanticweb.org/esther/ontologies/sys-self#Capability"/>
    </owl:ObjectProperty>
    


    <!-- http://www.semanticweb.org/esther/ontologies/sys-self#structures -->

    <owl:ObjectProperty rdf:about="http://www.semanticweb.org/esther/ontologies/sys-self#structures">
        <rdfs:domain rdf:resource="http://www.semanticweb.org/esther/ontologies/sys-self#Architecture"/>
        <rdfs:range rdf:resource="http://www.semanticweb.org/esther/ontologies/sys-self#Component"/>
    </owl:ObjectProperty>
    


    <!-- 
    ///////////////////////////////////////////////////////////////////////////////////////
    //
    // Classes
    //
    ///////////////////////////////////////////////////////////////////////////////////////
     -->

    


    <!-- http://www.semanticweb.org/esther/ontologies/sys-self#Action -->

    <owl:Class rdf:about="http://www.semanticweb.org/esther/ontologies/sys-self#Action">
        <rdfs:comment>Process of exerting a force or bringing about an effect that results from the capacity of an agent [Merriam-Webster]. 

A task is broken down into several individual actions.</rdfs:comment>
    </owl:Class>
    


    <!-- http://www.semanticweb.org/esther/ontologies/sys-self#Architecture -->

    <owl:Class rdf:about="http://www.semanticweb.org/esther/ontologies/sys-self#Architecture">
        <rdfs:comment>System Architecture is an abstract conceptualization, global, and focused to achieve the mission and life cycle concepts of the system. It describes a solution based on principles, concepts, and properties logically related to and consistent with each other.

It provides features, properties, and characteristics which satisfy, as far as possible, the problem or opportunity expressed by a set of system requirements (traceable to mission/business and stakeholder requirements) and life cycle concepts (e.g., operational, support) and which are implementable through technologies (e.g., mechanics, electronics, hydraulics, software, services, procedures, human activity).

It may also be applied to more than one system, in some cases forming the common structure, pattern, and set of requirements for classes or families of similar or related systems.

[SEBok]</rdfs:comment>
    </owl:Class>
    


    <!-- http://www.semanticweb.org/esther/ontologies/sys-self#Behavior -->

    <owl:Class rdf:about="http://www.semanticweb.org/esther/ontologies/sys-self#Behavior">
        <rdfs:comment>(1) Systems behavior is a change which leads to events in itself or other systems. Thus, action, reaction or response may constitute behavior in some cases. [Ackoff 1971]. This is the system science definition. Any system has behavior if its actions are in some way visible to systems around it. [SEBoK]

(2) The effect produced when an instance of a complex system or organism is used in its operational environment. This definition associates behavior with an emergent outcome of (complex) deployed system, more analogus to human/animal behavior. Taking this view, the whole organism has behavior but not any of its element systems; e.g., cars have behavior (when driven by people), engines have functions. [SEBoK]

We relate both perspectives by defining behavior as the way in which a system operates and interacts with its environment. This includes the observable actions and responses of the system as a whole.</rdfs:comment>
    </owl:Class>
    


    <!-- http://www.semanticweb.org/esther/ontologies/sys-self#Capability -->

    <owl:Class rdf:about="http://www.semanticweb.org/esther/ontologies/sys-self#Capability">
        <rdfs:comment>(1) The ability to achieve a desired effect under specified (performance) standards and conditions through combinations of ways and means (activities and resources) to perform a set of activities. [DoD 2009]

(2) An outcome or effect which can be achieved through use of features of a system of interest and which contributes to a desired benefit or goal. [SEBoK]

We define capability as the expected operational outcome (function) of the system that   satisfies a need under specified conditions with some (performance) standards.</rdfs:comment>
    </owl:Class>
    


    <!-- http://www.semanticweb.org/esther/ontologies/sys-self#Component -->

    <owl:Class rdf:about="http://www.semanticweb.org/esther/ontologies/sys-self#Component">
        <rdfs:comment>(1) An entity with discrete structure, such as an assembly or software module, within a system considered at a particular level of analysis. [ISO/IEC 1998]

(2) One of the parts that make up a system. [IEEE 2008]

(3) A set of functional services in the software, which, when implemented, represents a well-defined set of functions and is distinguishable by a unique name. [ISO/IEC 2008]

(4) In systems terms, we use component as the generic term for the level of decomposition at which system elements are no longer considered complex, and for which specialist design disciplines can be used. [SEBoK]</rdfs:comment>
    </owl:Class>
    


    <!-- http://www.semanticweb.org/esther/ontologies/sys-self#ComponentHW -->

    <owl:Class rdf:about="http://www.semanticweb.org/esther/ontologies/sys-self#ComponentHW">
        <rdfs:subClassOf rdf:resource="http://www.semanticweb.org/esther/ontologies/sys-self#Component"/>
    </owl:Class>
    


    <!-- http://www.semanticweb.org/esther/ontologies/sys-self#ComponentSW -->

    <owl:Class rdf:about="http://www.semanticweb.org/esther/ontologies/sys-self#ComponentSW">
        <rdfs:subClassOf rdf:resource="http://www.semanticweb.org/esther/ontologies/sys-self#Component"/>
    </owl:Class>
    


    <!-- http://www.semanticweb.org/esther/ontologies/sys-self#ComponentStatus -->

    <owl:Class rdf:about="http://www.semanticweb.org/esther/ontologies/sys-self#ComponentStatus"/>
    


    <!-- http://www.semanticweb.org/esther/ontologies/sys-self#Constraint -->

    <owl:Class rdf:about="http://www.semanticweb.org/esther/ontologies/sys-self#Constraint">
        <rdfs:comment>(1) A restriction, limit, or regulation imposed on a product, project, or process. [ANSI/EIA 1998]

(2) A type of requirement or design feature that cannot be traded off. [ANSI/EIA 1998]</rdfs:comment>
    </owl:Class>
    


    <!-- http://www.semanticweb.org/esther/ontologies/sys-self#Design -->

    <owl:Class rdf:about="http://www.semanticweb.org/esther/ontologies/sys-self#Design">
        <rdfs:comment>(1) Design includes activities to create concepts and models, and/or to conceive something (a system / a solution that answers an intended purpose) based on them; the outcome of design activities is a coherent and purposeful set of models or representations using defined constructs and patterns (that implement principles and concepts). [ISO/IEC/IEEC 2009]

(2.1) Design is the process of defining the architecture, components, interfaces, and other characteristics of a system or component; 
(2.2) Design is the process of defining the software architecture, components, modules, interfaces, and data for a software system to satisfy specified requirements;
[ISO/IEC/IEEE 24765:2010]</rdfs:comment>
    </owl:Class>
    


    <!-- http://www.semanticweb.org/esther/ontologies/sys-self#Environment -->

    <owl:Class rdf:about="http://www.semanticweb.org/esther/ontologies/sys-self#Environment">
        <rdfs:comment>(1) Anything affecting a subject system or affected by a subject system through interactions with it, or anything sharing an interpretation of interactions with a subject system. [IEEE 1175.1-2002 (R2007), 3.6]

(2) The surroundings (natural or man‐made) in which the system‐of-interest is utilized and supported; or in which the system is being developed, produced or retired. [INCOSE 2010]

(3) The operational environment is the environment in which systems are deployed. The problem or opportunity in response to which the system has been developed, exists in this environment. [SEBoK]

We define the environmnet as the operational surroundings of the system with which it interacts.</rdfs:comment>
    </owl:Class>
    


    <!-- http://www.semanticweb.org/esther/ontologies/sys-self#Goal -->

    <owl:Class rdf:about="http://www.semanticweb.org/esther/ontologies/sys-self#Goal">
        <rdfs:comment>A goal is a specific task achievable in a set time [SEBoK]</rdfs:comment>
    </owl:Class>
    


    <!-- http://www.semanticweb.org/esther/ontologies/sys-self#GoalStatus -->

    <owl:Class rdf:about="http://www.semanticweb.org/esther/ontologies/sys-self#GoalStatus">
        <rdfs:subClassOf rdf:resource="http://www.semanticweb.org/esther/ontologies/sys-self#Status"/>
    </owl:Class>
    


    <!-- http://www.semanticweb.org/esther/ontologies/sys-self#Interface -->

    <owl:Class rdf:about="http://www.semanticweb.org/esther/ontologies/sys-self#Interface">
        <rdfs:comment>(1) A shared boundary between two functional units, defined by various characteristics pertaining to the functions, physical signal exchanges, and other characteristics. [ISO/IEC 1993]

(2) A hardware or software component that connects two or more other components for the purpose of passing information from one to the other. [ISO/IEC 1993]

(3) To connect two or more components for the purpose of passing information from one to the other. [ISO/IEC/IEEE 2009]</rdfs:comment>
    </owl:Class>
    


    <!-- http://www.semanticweb.org/esther/ontologies/sys-self#MeasureOfEffectiveness -->

    <owl:Class rdf:about="http://www.semanticweb.org/esther/ontologies/sys-self#MeasureOfEffectiveness">
        <rdfs:subClassOf rdf:resource="http://www.semanticweb.org/esther/ontologies/sys-self#Metric"/>
        <rdfs:comment>The metrics by which an acquirer will measure satisfaction with products produced by the technical effort. [IEEE 2005]</rdfs:comment>
    </owl:Class>
    


    <!-- http://www.semanticweb.org/esther/ontologies/sys-self#MeasureOfPerformance -->

    <owl:Class rdf:about="http://www.semanticweb.org/esther/ontologies/sys-self#MeasureOfPerformance">
        <rdfs:subClassOf rdf:resource="http://www.semanticweb.org/esther/ontologies/sys-self#Metric"/>
        <rdfs:comment>An engineering performance measure that provides design requirements that are necessary to satisfy an MOE (measure of effectiveness). [IEEE 2005]</rdfs:comment>
    </owl:Class>
    


    <!-- http://www.semanticweb.org/esther/ontologies/sys-self#Metric -->

    <owl:Class rdf:about="http://www.semanticweb.org/esther/ontologies/sys-self#Metric">
        <rdfs:comment>Quantitative measure of the degree to which a system, component, or process possesses as given attribute.&quot; [ISO/IEC/IEEE 2010]</rdfs:comment>
    </owl:Class>
    


    <!-- http://www.semanticweb.org/esther/ontologies/sys-self#Mission -->

    <owl:Class rdf:about="http://www.semanticweb.org/esther/ontologies/sys-self#Mission">
        <rdfs:comment>The mission of a system is the top-level function of the system; the one that synthesizes all transformation of all inputs and solicitations into outputs and reactions. [SEBoK]

It is the result of the mission analysis, the set of concept definition activities. It examines the problem space and the needs of the business or enterprise and stakeholders. This activity focuses on the identification of the primary purpose(s) of the solution (its &quot;mission&quot;), while Stakeholder Needs and Requirements activity explores what capabilities stakeholders desire in accomplishing the mission and may include some detail on the performance of certain aspects of the solution. [SEBoK]</rdfs:comment>
    </owl:Class>
    


    <!-- http://www.semanticweb.org/esther/ontologies/sys-self#ObservableAction -->

    <owl:Class rdf:about="http://www.semanticweb.org/esther/ontologies/sys-self#ObservableAction">
        <rdfs:subClassOf rdf:resource="http://www.semanticweb.org/esther/ontologies/sys-self#Action"/>
    </owl:Class>
    


    <!-- http://www.semanticweb.org/esther/ontologies/sys-self#Requirement -->

    <owl:Class rdf:about="http://www.semanticweb.org/esther/ontologies/sys-self#Requirement">
        <rdfs:comment>(1a) A System Requirement is a statement that transforms the stakeholder, user-oriented view of desired capabilities into a technical view, of a solution that meets the operational needs of the user. [ISO/IEC/IEEE, 2015, section 6.4.2]

(1b) The System Requirement Definition process creates a set of measurable system requirements that specify, from the supplier’s perspective, what characteristics, attributes, and functional and performance requirements the system is to possess, in order to satisfy stakeholder requirements. [ISO/IEC/IEEE, 2015, section 6.4.2]

(2) The stakeholder requirements are defined for a system that can provide the services needed by users and other stakeholders in a defined environment. [ISO/IEC/IEEE, 2015, section 6.4.1]</rdfs:comment>
    </owl:Class>
    


    <!-- http://www.semanticweb.org/esther/ontologies/sys-self#Stakeholder -->

    <owl:Class rdf:about="http://www.semanticweb.org/esther/ontologies/sys-self#Stakeholder">
        <rdfs:comment>(1) Individual or organization having a right, share, claim, or interest in a system or in its possession of characteristics that meet their needs and expectations [ISO/IEC/IEEE 2015]

(2) An individual, team, or organization (or classes thereof) with interests in, or concerns relative to, a system. [ISO/IEC 2007]</rdfs:comment>
    </owl:Class>
    


    <!-- http://www.semanticweb.org/esther/ontologies/sys-self#State -->

    <owl:Class rdf:about="http://www.semanticweb.org/esther/ontologies/sys-self#State">
        <rdfs:comment>(1) The values of key system element qualities or properties at a given time. [Ackoff 1971]

(2) In Control Theory, the state variables are the smallest possible subset of system variables that can represent the entire state of the system at any given time. [Nise 2010]</rdfs:comment>
    </owl:Class>
    


    <!-- http://www.semanticweb.org/esther/ontologies/sys-self#Status -->

    <owl:Class rdf:about="http://www.semanticweb.org/esther/ontologies/sys-self#Status">
        <rdfs:comment>(1) state or condition with respect to circumstances [Merriam-Webster Dictionary]

For us, status is aligned with a description of the current or future potential, or health of the system. [Ackoff 1971, definition of state]</rdfs:comment>
    </owl:Class>
    


    <!-- http://www.semanticweb.org/esther/ontologies/sys-self#SystemStatus -->

    <owl:Class rdf:about="http://www.semanticweb.org/esther/ontologies/sys-self#SystemStatus">
        <rdfs:subClassOf rdf:resource="http://www.semanticweb.org/esther/ontologies/sys-self#Status"/>
    </owl:Class>
    


    <!-- http://www.semanticweb.org/esther/ontologies/sys-self#Task -->

    <owl:Class rdf:about="http://www.semanticweb.org/esther/ontologies/sys-self#Task">
        <rdfs:comment>In a robotic context, a task refers to a specific set of actions or operations that a robot is designed to perform to achieve a particular goal. Tasks can range from simple actions, such as picking up an object, to complex operations, such as assembling a product or navigating an environment.</rdfs:comment>
    </owl:Class>
    


    <!-- http://www.semanticweb.org/esther/ontologies/sys-self#TechnicalPerformanceMeasure -->

    <owl:Class rdf:about="http://www.semanticweb.org/esther/ontologies/sys-self#TechnicalPerformanceMeasure">
        <rdfs:subClassOf rdf:resource="http://www.semanticweb.org/esther/ontologies/sys-self#Metric"/>
        <rdfs:comment>(1) Measures of attributes of a system element within the system to determine how well the system or system element is satisfying specified requirements. [Roedler and Jones 2005, 1-65]

(2) A product design assessment, which estimates, through engineering analysis and tests, the values of essential performance parameters of the current design as effected by risk handling actions. [BMP 2012]</rdfs:comment>
    </owl:Class>
    


    <!-- http://www.semanticweb.org/esther/ontologies/sys-self#Value -->

    <owl:Class rdf:about="http://www.semanticweb.org/esther/ontologies/sys-self#Value">
        <rdfs:comment>In systems engineering we generally use the notion of &quot;value&quot; to describe the amount of benefit some thing, feature or capability provides to various stakeholders. It is an attribute of the problem space and considers the optimum set of requirements to deliver customer satisfaction. [SEBoK].</rdfs:comment>
    </owl:Class>
</rdf:RDF>



<!-- Generated by the OWL API (version 4.5.25.2023-02-15T19:15:49Z) https://github.com/owlcs/owlapi -->

